theories/ml_toy_lang/lang.v
@@ -197,7 +197,7 @@ Definition vals_compare_safe (vl v1 : val) : Prop :=
   val_is_unboxed vl ∨ val_is_unboxed v1.
 Global Arguments vals_compare_safe !_ !_ /.
 
-Definition state : Type := gmap loc (option (list val)).
+Local Notation state := (gmap loc (option (list val))).
 
 (** Equality and other typeclass stuff *)
 Lemma to_of_val v : to_val (of_val v) = Some v.
