theories/c_toy_lang/melocoton/primitive_laws.v
@@ -140,7 +140,7 @@ Context {p:prog_environ C_lang Σ}.
 Implicit Types P Q : iProp Σ.
 Implicit Types Φ Ψ : val → iProp Σ.
 Implicit Types efs : list expr.
-Implicit Types σ : state.
+Implicit Types σ : gmap loc heap_cell.
 Implicit Types v : val.
 Implicit Types l : loc.
 
